extra.v
@@ -1,0 +1,29 @@
+Require Import List.
+
+Fixpoint merge (l1 l2: list nat) : list nat :=
+  match l1, l2 with
+  | _, nil => l1
+  | nil, _ => l2
+  | h1::r1, h2::r2 => if Nat.leb h1 h2 then h1::h2::(merge r1 r2) 
+                                       else h2::h1::(merge r1 r2)
+  end.
+
+Fixpoint split (l : list nat) : (list nat)*(list nat) :=
+  match l with
+  | nil => (nil, nil)
+  | h::nil => (l, nil)
+  | h1::h2::r => match (split r) with
+                 | (l1, l2) => (h1::l1, h2::l2)
+                 end
+  end.
+
+
+Theorem sorted_red: forall (n:nat) (l: list nat), sorted(n::l) -> sorted l.
+Proof.
+ intros n l H.
+ inversion H. apply sorted0. assumption.
+Qed.
+
+
+
+Eval compute in (split (1::2::3::4::5::nil)).
